(WIP)

Reordering.v
@@ -1,6 +1,7 @@
 Require Import BinNat.
 Require Import Bool.
 Require Import List.
+Require Import sflib.
 
 Require Import Common.
 Require Import Lang.
@@ -43,38 +44,200 @@ Definition inst_locates_at (md:Ir.IRModule.t) (c:Ir.Config.t) (i1 i2:Ir.Inst.t):
     Some c' = incrpc' md c /\
     Ir.Config.cur_inst md c' = Some i2.
 
+
+Lemma cur_fdef_pc_update_pc:
+  forall md c p fdef p0
+         (HPREV:Ir.Config.cur_fdef_pc md c = Some (fdef, p0)),
+    Ir.Config.cur_fdef_pc md (Ir.Config.update_pc c p) = Some (fdef, p).
+Proof.
+  intros.
+  unfold Ir.Config.cur_fdef_pc in *.
+  unfold Ir.Config.update_pc.
+  des_ifs; simpl in *; inversion Heq; rewrite H0 in *;
+    unfold Ir.Config.get_funid in *;
+    unfold Ir.Config.cid_to_f in *; congruence.
+Qed.
+    
+Lemma cur_fdef_pc_update_rval:
+  forall md c r v,
+    Ir.Config.cur_fdef_pc md (Ir.Config.update_rval c r v) =
+         Ir.Config.cur_fdef_pc md c.
+Proof.
+  intros.
+  unfold Ir.Config.cur_fdef_pc.
+  unfold Ir.Config.update_rval.
+  des_ifs; try congruence;
+  try(simpl in *; inv Heq; unfold Ir.Config.get_funid in *; simpl in *;
+    congruence).
+Qed.
+
+Lemma incrpc_update_rval:
+  forall md st r v,
+    Ir.SmallStep.incrpc md (Ir.Config.update_rval st r v) =
+    Ir.Config.update_rval (Ir.SmallStep.incrpc md st) r v.
+Proof.
+  intros.
+  unfold Ir.SmallStep.incrpc.
+  rewrite cur_fdef_pc_update_rval.
+  des_ifs.
+  unfold Ir.Config.update_rval.
+  destruct (Ir.Config.s st) eqn:Hs.
+  - unfold Ir.Config.update_pc at 2. repeat (rewrite Hs). reflexivity.
+  - unfold Ir.Config.update_pc at 2. repeat (rewrite Hs).
+    destruct p1 eqn:Hp1.
+    destruct p2 eqn:Hp2.
+    simpl. unfold Ir.Config.update_pc at 1. simpl.
+    unfold Ir.Config.update_pc. repeat (rewrite Hs). simpl.
+    reflexivity.
+Qed.
+
+Lemma cur_inst_update_reg_and_incrpc:
+  forall md st r v,
+    Ir.Config.cur_inst md (Ir.SmallStep.update_reg_and_incrpc md st r v) =
+    Ir.Config.cur_inst md (Ir.SmallStep.incrpc md st).
+Proof.
+  intros.
+  unfold Ir.Config.cur_inst.
+  unfold Ir.SmallStep.update_reg_and_incrpc.
+  rewrite incrpc_update_rval.
+  rewrite cur_fdef_pc_update_rval.
+  reflexivity.
+Qed.
+
+Lemma incrpc'_incrpc:
+  forall md st st'
+         (HINCRPC':Some st' = incrpc' md st),
+    st' = Ir.SmallStep.incrpc md st.
+Proof.
+  intros.
+  unfold incrpc' in *.
+  unfold Ir.SmallStep.incrpc.
+  des_ifs.
+Qed.
+
+Lemma m_update_reg_and_incrpc:
+  forall md st r v,
+    Ir.Config.m (Ir.SmallStep.update_reg_and_incrpc md st r v) =
+    Ir.Config.m st.
+Proof.
+  intros.
+  unfold Ir.SmallStep.update_reg_and_incrpc.
+  unfold Ir.SmallStep.incrpc.
+  unfold Ir.Config.update_pc.
+  unfold Ir.Config.update_rval.
+  des_ifs.
+Qed.
+
+Lemma get_val_incrpc:
+  forall md st op,
+    Ir.Config.get_val (Ir.SmallStep.incrpc md st) op = Ir.Config.get_val st op.
+Proof.
+  intros.
+  unfold Ir.SmallStep.incrpc.
+  unfold Ir.Config.get_val.
+  des_ifs.
+  unfold Ir.Config.update_pc.
+  des_ifs.
+  unfold Ir.Config.get_rval.
+  simpl. rewrite Heq1. reflexivity.
+Qed.
+
+Lemma get_val_independent:
+  forall r1 r2 (HNEQ:r1 <> r2) md st v,
+    Ir.Config.get_val (Ir.SmallStep.update_reg_and_incrpc md st r2 v) (Ir.opreg r1) =
+    Ir.Config.get_val st (Ir.opreg r1).
+Proof.
+  intros.
+  unfold Ir.SmallStep.update_reg_and_incrpc.
+  rewrite get_val_incrpc.
+  unfold Ir.Config.get_val.
+  unfold Ir.Config.update_rval.
+  unfold Ir.Config.get_rval.
+  des_ifs.
+  congruence. simpl in Heq. inv Heq.
+  unfold Ir.Regfile.update. unfold Ir.Regfile.get.
+  simpl. apply not_eq_sym in HNEQ. rewrite <- PeanoNat.Nat.eqb_neq in HNEQ.
+  rewrite HNEQ. reflexivity.
+Qed.
+
+Lemma config_eq_refl:
+  forall md st
+         
+    Ir.Config.eq (Ir.SmallStep.incrpc 
+      (Ir.SmallStep.update_reg_and_incrpc md
+        (Ir.SmallStep.update_reg_and_incrpc md st r1 v1) r2 v2)
+      (Ir.SmallStep.update_reg_and_incrpc md
+        (Ir.SmallStep.update_reg_and_incrpc md st r2 v2) r1 v1).
+
+Lemma config_eq_update_reg_and_incrpc:
+  forall md st r1 r2 v1 v2
+         (HNEQ:r2 <> r1),
+    Ir.Config.eq
+      (Ir.SmallStep.update_reg_and_incrpc md
+        (Ir.SmallStep.update_reg_and_incrpc md st r1 v1) r2 v2)
+      (Ir.SmallStep.update_reg_and_incrpc md
+        (Ir.SmallStep.update_reg_and_incrpc md st r2 v2) r1 v1).
+Proof.
+  intros.
+  
+
+
 Inductive nstep_eq: (Ir.trace * Ir.SmallStep.step_res) ->
                     (Ir.trace * Ir.SmallStep.step_res) -> Prop :=
 | nseq_goes_wrong:
-    forall (t:Ir.trace),
-      nstep_eq (t, (Ir.SmallStep.sr_goes_wrong)) (t, (Ir.SmallStep.sr_goes_wrong))
+    forall (t1 t2:Ir.trace)
+        (HEQ:List.filter Ir.not_none t1 = List.filter Ir.not_none t2),
+      nstep_eq (t1, (Ir.SmallStep.sr_goes_wrong)) (t2, (Ir.SmallStep.sr_goes_wrong))
 | nseq_oom:
-    forall (t:Ir.trace),
-      nstep_eq (t, (Ir.SmallStep.sr_oom)) (t, (Ir.SmallStep.sr_oom))
+    forall (t1 t2:Ir.trace)
+        (HEQ:List.filter Ir.not_none t1 = List.filter Ir.not_none t2),
+      nstep_eq (t1, (Ir.SmallStep.sr_oom)) (t2, (Ir.SmallStep.sr_oom))
 | nseq_prog_finish:
-    forall (t:Ir.trace) v,
-      nstep_eq (t, (Ir.SmallStep.sr_prog_finish v)) (t, (Ir.SmallStep.sr_prog_finish v))
+    forall (t1 t2:Ir.trace) v
+        (HEQ:List.filter Ir.not_none t1 = List.filter Ir.not_none t2),
+      nstep_eq (t1, (Ir.SmallStep.sr_prog_finish v)) (t2, (Ir.SmallStep.sr_prog_finish v))
 | nseq_success:
-    forall (t:Ir.trace) e c,
-      nstep_eq (t, (Ir.SmallStep.sr_success e c))
-               (t, (Ir.SmallStep.sr_success e c)).
+    forall (t1 t2:Ir.trace) e c
+        (HEQ:List.filter Ir.not_none t1 = List.filter Ir.not_none t2),
+      nstep_eq (t1, (Ir.SmallStep.sr_success e c))
+               (t2, (Ir.SmallStep.sr_success e c)).
 
 (* Is it valid to reorder 'i1;i2' into 'i2;i1'? *)
-Definition inst_reorderable (i1 i2:Ir.Inst.t): Prop :=
+Definition inst_reordering_valid (i1 i2:Ir.Inst.t): Prop :=
   (* If there's no data dependency from i1 to i2 *)
   forall (HNODEP:has_data_dependency i1 i2 = false),
     (* 'i1;i2' -> 'i2;i1' is allowed *)
-    forall (md:Ir.IRModule.t) (* Module *)
+    forall (md md':Ir.IRModule.t) (* IR Modules *)
            (st:Ir.Config.t) (* Initial state *)
-           (HWF:Ir.Config.wf md st) (* Well-formedness of st0 *)
+           (HWF:Ir.Config.wf md st) (* Well-formedness of st *)
            (HLOCATE:inst_locates_at md st i1 i2)
+           (HLOCATE':inst_locates_at md' st i2 i1)
            (sr:Ir.trace * Ir.SmallStep.step_res)
            (HSTEP:Ir.SmallStep.inst_nstep md st 2 sr),
-      exists md' (* Reordered IRModule *)
-             sr', (* step result after 'i2;i1' *)
-        inst_locates_at md' st i2 i1 /\ (* Reordered *)
+      exists sr', (* step result after 'i2;i1' *)
         Ir.SmallStep.inst_nstep md' st 2 sr' /\
         nstep_eq sr sr'.
+
+
+(* If instruction i does not change memory, it does not raise OOM. *)
+Lemma no_mem_change_no_oom:
+  forall i st md
+         (HNOMEMCHG:Ir.SmallStep.changes_mem i = false)
+         (HINST:Ir.Config.cur_inst md st = Some i)
+         (HOOM:Ir.SmallStep.inst_step md st Ir.SmallStep.sr_oom),
+    False.
+Proof.
+  intros.
+  inversion HOOM.
+  - unfold Ir.SmallStep.inst_det_step in HNEXT.
+    rewrite HINST in HNEXT.
+    destruct i; des_ifs.
+  - rewrite HINST in HCUR.
+    inversion HCUR. rewrite HINST0 in H1.
+    rewrite <- H1 in HNOMEMCHG. inversion HNOMEMCHG.
+Qed.
+
+
 
 (* Reordering between ptrtoint/ptrtoint:
 
@@ -84,14 +247,114 @@ Definition inst_reorderable (i1 i2:Ir.Inst.t): Prop :=
    r2 = ptrtoint opptr2 ty2;
    r1 = ptrtoint opptr1 ty1
 *)
-(*
-Lemma reorder_unidir_ptrtoint_ptrtoint:
+Lemma reorder_ptrtoint_ptrtoint:
   forall i1 i2 r1 r2 opptr1 opptr2 ty1 ty2
          (HINST1:i1 = Ir.Inst.iptrtoint r1 opptr1 ty1)
          (HINST2:i2 = Ir.Inst.iptrtoint r2 opptr2 ty2),
-    inst_reorderable_unidir i1 i2.
-*)
-  
+    inst_reordering_valid i1 i2.
+Proof.
+  intros.
+  assert (HNOMEMCHG1:Ir.SmallStep.changes_mem i1 = false).
+  { rewrite HINST1. reflexivity. }
+  assert (HNOMEMCHG2:Ir.SmallStep.changes_mem i2 = false).
+  { rewrite HINST2. reflexivity. }
+
+  unfold inst_reordering_valid.
+  intros.
+  unfold has_data_dependency in HNODEP.
+  rewrite HINST1, HINST2 in HNODEP.
+  unfold Ir.Inst.regops in HNODEP.
+  unfold Ir.regop in HNODEP.
+  simpl in HNODEP.
+
+  unfold inst_locates_at in *.
+  destruct HLOCATE as [st_next [HLOCATE1 [HLOCATE_NEXT HLOCATE2]]].
+  destruct HLOCATE' as [st_next' [HLOCATE1' [HLOCATE_NEXT' HLOCATE2']]].
+  inv HSTEP.
+  - inv HSUCC.
+    + inv HSINGLE0; try congruence.
+      unfold Ir.SmallStep.inst_det_step in HNEXT.
+      des_ifs.
+      * inv HSINGLE; try (rewrite cur_inst_update_reg_and_incrpc in *;
+           apply incrpc'_incrpc in HLOCATE_NEXT;
+           congruence).
+        unfold Ir.SmallStep.inst_det_step in HNEXT.
+        rewrite cur_inst_update_reg_and_incrpc in *.
+        apply incrpc'_incrpc in HLOCATE_NEXT.
+        rewrite HLOCATE_NEXT in HLOCATE2.
+        rewrite HLOCATE2 in HNEXT.
+        des_ifs.
+        { (* i2 is ptrtoint <const(int)>. *)
+          exists (nil, Ir.SmallStep.sr_goes_wrong).
+          split.
+          - eapply Ir.SmallStep.ns_goes_wrong.
+            eapply Ir.SmallStep.ns_one.
+            constructor. 
+            unfold Ir.SmallStep.inst_det_step.
+            rewrite HLOCATE1'.
+            unfold Ir.Config.get_val in *. inv Heq1. rewrite H0.
+            reflexivity.
+          - apply nseq_goes_wrong. reflexivity.
+        }
+        { (* i2 is ptrtoint <const(ptr)>. *)
+          rewrite m_update_reg_and_incrpc.
+          (* Needs to know that r1 != r2! from SSA property. *)
+          eexists.
+          split.
+          - eapply Ir.SmallStep.ns_success.
+            eapply Ir.SmallStep.ns_one.
+            econstructor.
+            unfold Ir.SmallStep.inst_det_step.
+            rewrite HLOCATE1'. unfold Ir.Config.get_val in *. inv Heq1. rewrite H0.
+            reflexivity.
+            econstructor.
+            unfold Ir.SmallStep.inst_det_step.
+            rewrite cur_inst_update_reg_and_incrpc.
+            apply incrpc'_incrpc in HLOCATE_NEXT'.
+            rewrite HLOCATE_NEXT' in HLOCATE2'.
+            rewrite HLOCATE2'.
+            destruct opptr1. (* when i1's operand is constant *)
+            + unfold Ir.Config.get_val in *. inv Heq0. rewrite H0.
+              reflexivity.
+            + rewrite get_val_independent. rewrite Heq0. reflexivity.
+              admit. (* SSA property!! *)
+          - rewrite m_update_reg_and_incrpc.
+      
+inv HOOM.
+    + inv HOOM0.
+    + inv HSUCC.
+      exfalso. eapply no_mem_change_no_oom.
+      rewrite HNOMEMCHG1. reflexivity.
+      eapply HLOCATE1. assumption.
+  - inv HGW.
+    + inv HGW0.
+    + inv HSUCC.
+      exists (Ir.e_none::nil, Ir.SmallStep.sr_goes_wrong).
+      split.
+      * eapply Ir.SmallStep.ns_success.
+        eapply Ir.SmallStep.ns_success.
+
+
+ Ir.Config.cur_inst md
+           (Ir.SmallStep.update_reg_and_incrpc md st r1
+              (Value.Ir.num (Ir.SmallStep.p2N p (Ir.Config.m st) n
+        
+        apply Ir.SmallStep.ns_success with (c' := c').
+        constructor.
+        
+        
+      inversion HSUCC.
+      inversion HSINGLE.
+      * inversion HSUCC.
+        -- rewrite <- H12 in *. clear H12.
+           unfold Ir.SmallStep.inst_det_step in HNEXT.
+           rewrite HLOCATE1 in HNEXT.
+
+Ltac des_op c op op' HINV :=
+  destruct (Ir.Config.get_val c op) as [op' | ]; try (inversion HINV; fail).
+Ltac des_inv v HINV :=
+  destruct (v); try (inversion HINV; fail).
+
 
 End Reordering.
 
